Hotfix (now compiles)

backend/StackingproofC.v
@@ -713,6 +713,126 @@ End STACKINGEXTRA.
 
 
 
+
+Section LIFT.
+
+Require Import Program.Equality.
+
+Definition wf_tgt (st_tgt0: Mach.state): Prop :=
+  exists parent_sp parent_ra, last_option st_tgt0.(MachC.get_stack) = Some (MachC.dummy_stack parent_sp parent_ra)
+.
+
+Lemma lift_starN
+      rao
+      cnt tse tge st_tgt0 tr st_tgt1
+      (STAR: starN (Mach.step rao) tse tge cnt st_tgt0 tr st_tgt1)
+      (DUMMYTGT: wf_tgt st_tgt0)
+      (STKAFTER: get_stack st_tgt1 <> [])
+  :
+    <<STAR: starN (step rao) tse tge cnt st_tgt0 tr st_tgt1>>
+.
+Proof.
+  unfold wf_tgt in *.
+  induction STAR; ii; ss.
+  { econs; et. }
+  pose s as S1. pose s' as S2. pose s'' as S3.
+  (* pose s1 as S1. pose s2 as S2. pose s3 as S3. *)
+  econs; et.
+  - econs; et.
+    des. inv H; ss; destruct s0; ss. exfalso. clarify.
+    clear - STAR STKAFTER.
+    dependent induction STAR; ii; ss. inv H; ss.
+  - des. exploit IHSTAR; et. inv H; ss; try (by esplits; et).
+    + des_ifs. rewrite DUMMYTGT. esplits; et.
+    + des_ifs.
+      * ss. clarify.
+        clear - STAR STKAFTER.
+        dependent induction STAR; ii; ss. inv H; ss.
+      * rewrite DUMMYTGT. esplits; et.
+Qed.
+
+Lemma lift_starN_stronger
+      rao
+      cnt tse tge st_tgt0 tr st_tgt1
+      (STAR: starN (Mach.step rao) tse tge cnt st_tgt0 tr st_tgt1)
+      (DUMMYTGT: wf_tgt st_tgt0)
+      (STKAFTER: get_stack st_tgt1 <> [])
+  :
+    <<STAR: starN (step rao) tse tge cnt st_tgt0 tr st_tgt1>> /\ <<DUMMYTGT: wf_tgt st_tgt1>>
+.
+Proof.
+  unfold wf_tgt in *.
+  revert_until STAR.
+  induction STAR; ii; ss.
+  { split. - econs; et. - des. esplits; et. }
+  assert(DUMMYTGT0: wf_tgt s'').
+  { clarify.
+    eapply IHSTAR; et. clear IHSTAR.
+    des. inv H; ss; try (by esplits; et).
+    - des_ifs. esplits; et.
+    - des_ifs.
+      + ss. clarify. inv STAR; ss. inv H; ss.
+      + esplits; et.
+  }
+  split; ss.
+  econs; et.
+  - econs; et.
+    des. inv H; ss; destruct s0; ss. exfalso. clarify. ss. clarify.
+    clear - STAR STKAFTER.
+    dependent induction STAR; ii; ss. inv H; ss.
+  - des.
+    exploit IHSTAR; et.
+    { inv H; ss; try (by esplits; et).
+      - des_ifs. esplits; et.
+      - des_ifs.
+        + ss. clarify. inv STAR; ss. inv H; ss.
+        + esplits; et.
+    }
+    i; des.
+    inv H; ss; try (by esplits; et).
+Qed.
+
+Lemma starN_plus_iff
+      G ST (step: Senv.t -> G -> ST -> trace -> ST -> Prop) se ge st0 tr st1
+  :
+    (exists n, starN step se ge n st0 tr st1 /\ (n > 0)%nat) <-> plus step se ge st0 tr st1
+.
+Proof.
+  split; i; des.
+  - destruct n; ss.
+    { xomega. }
+    ginduction H; ii; ss.
+    { xomega. }
+    clarify. inv H0.
+    + eapply plus_star_trans; et.
+      { apply plus_one; et. }
+      { apply star_refl; et. }
+    + eapply plus_trans; et.
+      { apply plus_one; et. }
+      eapply IHstarN; et. xomega.
+  - inv H. apply star_starN in H1. des. exists (Datatypes.S n). esplits; et.
+    { econs; et. }
+    { xomega. }
+Qed.
+
+Lemma lift_plus
+      rao
+      tse tge st_tgt0 tr st_tgt1
+      (PLUS: plus (Mach.step rao) tse tge st_tgt0 tr st_tgt1)
+      (DUMMYTGT: wf_tgt st_tgt0)
+      (STKAFTER: get_stack st_tgt1 <> [])
+  :
+    <<PLUS: plus (step rao) tse tge st_tgt0 tr st_tgt1>> /\ <<DUMMYTGT: wf_tgt st_tgt1>>
+.
+Proof.
+  apply starN_plus_iff in PLUS. des. apply lift_starN_stronger in PLUS; et. des. esplits; et.
+  apply starN_plus_iff; et.
+Qed.
+
+End LIFT.
+
+
+
 Lemma external_call_parallel_rule:
   forall (F V: Type) ef (ge: Genv.t F V) vargs1 m1 t vres1 m1' m2 j P vargs2,
   external_call ef ge vargs1 m1 t vres1 m1' ->
@@ -1404,6 +1524,7 @@ Inductive match_states
                    <<EQ: dummy_stack_src.(current_locset) (R mr) = st_tgt0.(init_rs) mr>>
                    /\ <<PTRFREE: ~ is_real_ptr (st_tgt0.(init_rs) mr)>>>> /\
         <<SIG: dummy_stack_src.(current_function).(Linear.fn_sig) = st_tgt0.(init_sg)>>)
+    (WFTGT: wf_tgt st_tgt0.(MachC.st))
 .
 
 Inductive match_states_at
@@ -1606,6 +1727,7 @@ Proof.
           + i. ss. split.
             * erewrite OUT; ss. ii. hexpl loc_arguments_acceptable_2 ACCP. ss. clarify.
             * eapply PTRFREE. ii. hexpl loc_arguments_acceptable_2 ACCP. ss. clarify.
+        - rr. ss. esplits; eauto.
       }
     }
   - (* init progress *)
@@ -2021,6 +2143,9 @@ Proof.
     { des. et. }
     i; des.
     destruct st_tgt0. ss. folder.
+    exploit lift_plus; eauto.
+    { ii. inv STEPSRC. inv H0; ss; try inv STACKS; ss; clarify; et. }
+    i; des.
     esplits; eauto.
     + left.
       eapply spread_dplus; et.
